Trying to rework FreeRTOS proof to use memory layout

timing/examples/FreeRTOS_tasks_noasserts_proofs_clz.v
@@ -3,6 +3,9 @@ Require Import riscvTiming.
 Import RISCVNotations.
 Require Import memsolve.
 Require Import Lia.
+Require Import List.
+Import ListNotations.
+Open Scope list_scope.
 
 (* Some machinery describing the CPU *)
 Variable ML : N.
@@ -29,7 +32,7 @@ Definition time_branch : N :=
    - Modifying shared memory
    - Performance optimization
 *)
-Definition uxSchedulerSuspended (gp : N) (mem : addr -> N) : N :=
+Definition uxSchedulerSuspended (gp : N) (mem : memory) : N :=
     mem Ⓓ[gp ⊖ 1952].
 
 (* The address of the doubleword in static memory that is nonzero when a task is
@@ -42,13 +45,13 @@ Definition addr_xYieldPendings (gp : N) : addr :=
 (* A pointer in static memory to the Current Task Control Block (TCB). The TCB
    is a data structure containing all essential information for managing a task.
 *)
-Definition pxCurrentTCB (gp : N) (mem : addr -> N) : N :=
+Definition pxCurrentTCB (gp : N) (mem : memory) : N :=
     mem Ⓓ[gp ⊖ 1896].
 
 (* The doubleword in static memory that records the highest priority out of all
    currently-ready tasks.
 *)
-Definition uxTopReadyPriority (gp : N) (mem : addr -> N) : N :=
+Definition uxTopReadyPriority (gp : N) (mem : memory) : N :=
     mem Ⓓ[gp ⊖ 1920].
 
 (* The address in static memory of a list of linked-lists that record all currently-
@@ -111,27 +114,40 @@ Definition gp_sp_noverlap (gp sp : N) : Prop :=
 (* These two definitions state that any two of the above buffers we're interested
    in do not overlap
 *)
-Definition static_buffer_lengths_in_bytes (a : addr) : option N :=
-    match a with
-    (* uxSchedulerSuspended *)
-    | 1952
-    (* xYieldPendings*)
-    | 1932 
-    (* pxCurrentTCB *)
-    | 1896 
-    (* uxTopReadyPriority *)
-    | 1920 => Some 4
-    | _ => None
-    end.
 
-Definition smem_well_formed (gp : N) : Prop :=
-    forall x y len_x len_y,
-                x <> y ->
-                static_buffer_lengths_in_bytes x = Some len_x ->
-                static_buffer_lengths_in_bytes y = Some len_y ->
-            ~ overlap 32
-                (gp ⊖ x) len_x
-                (gp ⊖ y) len_y.
+Definition non_overlapping_smem_layout (gp : N) (mem : memory) : list (N * N) :=
+    [
+        (gp ⊖ 920 ⊕ (31 ⊖ clz (uxTopReadyPriority gp mem) 32) * 20, 4);
+        (gp ⊖ 1952, 4); (* uxSchedulerSuspended *)
+        (gp ⊖ 1932, 4); (* xYieldPendings*)
+        (gp ⊖ 1896, 4); (* pxCurrentTCB *)
+        (gp ⊖ 1920, 4) (* uxTopReadyPriority *)
+    ].
+Definition smem_well_formed (gp : N) (mem : memory) : Prop :=
+    forall x xw y yw,
+        x <> y ->
+        In (x, xw) (non_overlapping_smem_layout gp mem) ->
+        In (y, yw) (non_overlapping_smem_layout gp mem) ->
+        ~ overlap 32 x xw y yw.
+
+Definition non_overlapping_mem_layout (mem : memory) (gp sp : N) : list (N * N) :=
+    [
+        (gp ⊖ __global_size, __global_size);
+        (sp ⊖ vTaskSwitchContext_stack_frame_size, vTaskSwitchContext_stack_frame_size);
+        (48 + pxCurrentTCB gp mem, 4);
+        (mem Ⓓ[48 + pxCurrentTCB gp mem], 4);
+        (8 + mem Ⓓ[48 + pxCurrentTCB gp mem], 4);
+        (12 + mem Ⓓ[48 + pxCurrentTCB gp mem], 4);
+        (4 + mem Ⓓ[gp ⊖ 920 ⊕ (31 ⊖ clz (uxTopReadyPriority gp mem) 32) * 20], 4);
+        (4 + mem Ⓓ[ 4 + mem Ⓓ[gp ⊖ 920 ⊕ (31 ⊖ clz (uxTopReadyPriority gp mem) 32) * 20] ], 4)
+    ].
+Definition memory_well_formed (gp sp : N) (mem : memory) :=
+    smem_well_formed gp mem /\
+        forall x xw y yw,
+            x <> y ->
+            In (x, xw) (non_overlapping_mem_layout mem gp sp) ->
+            In (y, yw) (non_overlapping_mem_layout mem gp sp) ->
+            ~ overlap 32 x xw y yw.
 
 (* I don't yet know the significance of the address
       gp ⊖ 920 ⊕ (31 ⊖ clz (uxTopReadyPriority gp mem) 32) * 20
@@ -139,88 +155,88 @@ Definition smem_well_formed (gp : N) : Prop :=
    TCB or stack memory. Some of these assumptions can actually be proven due to 
    the boundaries of clz (count leading zeroes) being 0..32
 *)
-Definition pxCurrentTCB_noverlap_clz_static (gp : N) (mem : addr -> N) : Prop :=
+(* Definition pxCurrentTCB_noverlap_clz_static (gp : N) (mem : memory) : Prop :=
     ~ overlap 32
         (48 + pxCurrentTCB gp mem) 4
-        (gp ⊖ 920 ⊕ (31 ⊖ clz (uxTopReadyPriority gp mem) 32) * 20) 4.
+        (gp ⊖ 920 ⊕ (31 ⊖ clz (uxTopReadyPriority gp mem) 32) * 20) 4. *)
 
-Definition clz_noverlap_smem (gp : N) mem : Prop :=
+(* Definition clz_noverlap_smem (gp : N) mem : Prop :=
     forall x len_x,
         static_buffer_lengths_in_bytes x = Some len_x ->
         ~ overlap 32
             (gp ⊖ x) len_x
-            (gp ⊖ 920 ⊕ (31 ⊖ clz (uxTopReadyPriority gp mem) 32) * 20) 4.
+            (gp ⊖ 920 ⊕ (31 ⊖ clz (uxTopReadyPriority gp mem) 32) * 20) 4. *)
 
 (* The TCB doesn't overlap static memory or the stack frame *)
-Definition pxCurrentTCB_noverlap_static (gp : N) (mem : addr -> N) : Prop :=
+(* Definition pxCurrentTCB_noverlap_static (gp : N) (mem : memory) : Prop :=
     forall x len_x,
         static_buffer_lengths_in_bytes x = Some len_x ->
         ~ overlap 32
             (48 + pxCurrentTCB gp mem) 4
-            (gp ⊖ x) len_x.
+            (gp ⊖ x) len_x. *)
 
-Definition pxCurrentTCB_noverlap_stackframe (gp base_sp : N) (mem : addr -> N) : Prop :=
+(* Definition pxCurrentTCB_noverlap_stackframe (gp base_sp : N) (mem : memory) : Prop :=
     ~ overlap 32
         (48 + pxCurrentTCB gp mem) 4
-        (base_sp ⊖ 16) 16.
+        (base_sp ⊖ 16) 16. *)
 
 (* The address contained in the current TCB doesn't overlap with static memory
    or the stack frame *)
-Definition mem_pxCurrentTCB_noverlap_stackframe (gp base_sp : N) (mem : addr -> N) : Prop :=
+(* Definition mem_pxCurrentTCB_noverlap_stackframe (gp base_sp : N) (mem : memory) : Prop :=
     ~ overlap 32
         (mem Ⓓ[48 + pxCurrentTCB gp mem]) 4
-        (base_sp ⊖ 16) 16.
+        (base_sp ⊖ 16) 16. *)
 
-Definition mem_pxCurrentTCB_noverlap_static (gp : N) (mem : addr -> N) : Prop :=
+(* Definition mem_pxCurrentTCB_noverlap_static (gp : N) (mem : memory) : Prop :=
     forall x len_x,
         static_buffer_lengths_in_bytes x = Some len_x ->
         ~ overlap 32
             (mem Ⓓ[48 + pxCurrentTCB gp mem]) 4
-            (gp ⊖ x) len_x.
+            (gp ⊖ x) len_x. *)
 
 (* Offsets into the address contained in the current TCB don't overlap with 
    the clz address or stack memory *)
-Definition offset_mem_pxCurrentTCB_noverlap_clz (gp : N) (mem : addr -> N) : Prop :=
+(* Definition offset_mem_pxCurrentTCB_noverlap_clz (gp : N) (mem : memory) : Prop :=
     forall k, k = 8 \/ k = 12 ->
         ~ overlap 32
             (k + mem Ⓓ[48 + pxCurrentTCB gp mem]) 4
             (gp ⊖ 920 ⊕ (31 ⊖ clz (uxTopReadyPriority gp mem) 32) * 20) 4.
 
-Definition clz_noverlap_sframe (gp base_sp : N) (mem : addr -> N) : Prop :=
+Definition clz_noverlap_sframe (gp base_sp : N) (mem : memory) : Prop :=
     ~ overlap 32 
         (base_sp ⊖ 16) 16
-        (gp ⊖ 920 ⊕ (31 ⊖ clz (uxTopReadyPriority gp mem) 32) * 20) 4.
+        (gp ⊖ 920 ⊕ (31 ⊖ clz (uxTopReadyPriority gp mem) 32) * 20) 4. *)
 
 (* An offset into the buffer at the clz address doesn't overlap with static
    memory or the stack frame *)
-Definition mem4_pxCurrentTCB_noverlap_stackframe (gp base_sp : N) (mem : addr -> N) : Prop :=
+(* Definition mem4_pxCurrentTCB_noverlap_stackframe (gp base_sp : N) (mem : memory) : Prop :=
         ~ overlap 32
         (base_sp ⊖ 16) 16
             (4 + mem Ⓓ[gp ⊖ 920 ⊕ (31 ⊖ clz (uxTopReadyPriority gp mem) 32) * 20]) 4.
 
-Definition mem4_pxCurrentTCB_noverlap_static (gp : N) (mem : addr -> N) : Prop :=
+Definition mem4_pxCurrentTCB_noverlap_static (gp : N) (mem : memory) : Prop :=
     forall x len_x,
         static_buffer_lengths_in_bytes x = Some len_x ->
         ~ overlap 32
             (gp ⊖ x) 4
-            (4 + mem Ⓓ[gp ⊖ 920 ⊕ (31 ⊖ clz (uxTopReadyPriority gp mem) 32) * 20]) 4.
+            (4 + mem Ⓓ[gp ⊖ 920 ⊕ (31 ⊖ clz (uxTopReadyPriority gp mem) 32) * 20]) 4. *)
 
 (* An offset into the buffer at an offset into the buffer at the clz address 
    doesn't overlap with static memory or the stack frame *)
-Definition mem4_mem4_noverlap_stackframe (gp base_sp : N) (mem : addr -> N) :=
+(* Definition mem4_mem4_noverlap_stackframe (gp base_sp : N) (mem : memory) :=
     ~ overlap 32
         (base_sp ⊖ 16) 16
         (4 + mem Ⓓ[ 4 + mem Ⓓ[ gp ⊖ 920 ⊕ (31 ⊖ clz (uxTopReadyPriority gp mem) 32) * 20 ] ]) 4.
 
-Definition mem4_mem4_noverlap_static (gp : N) (mem : addr -> N) :=
+Definition mem4_mem4_noverlap_static (gp : N) (mem : memory) :=
     forall x len_x,
         static_buffer_lengths_in_bytes x = Some len_x ->
         ~ overlap 32
             (gp ⊖ x) 4
-            (4 + mem Ⓓ[ 4 + mem Ⓓ[ gp ⊖ 920 ⊕ (31 ⊖ clz (uxTopReadyPriority gp mem) 32) * 20 ] ]) 4.
+            (4 + mem Ⓓ[ 4 + mem Ⓓ[ gp ⊖ 920 ⊕ (31 ⊖ clz (uxTopReadyPriority gp mem) 32) * 20 ] ]) 4. *)
 
 (* Stick them all together *)
-Definition common_noverlaps gp base_sp mem : Prop :=
+(* Definition common_noverlaps gp base_sp mem : Prop :=
     gp_sp_noverlap gp base_sp /\
     smem_well_formed gp /\
     pxCurrentTCB_noverlap_static gp mem /\
@@ -232,9 +248,9 @@ Definition common_noverlaps gp base_sp mem : Prop :=
     offset_mem_pxCurrentTCB_noverlap_clz gp mem /\
     clz_noverlap_sframe gp base_sp mem /\
     mem4_pxCurrentTCB_noverlap_stackframe gp base_sp mem /\
-    mem4_pxCurrentTCB_noverlap_static gp mem.
+    mem4_pxCurrentTCB_noverlap_static gp mem. *)
 
-Definition time_of_vTaskSwitchContext (t : trace) (gp : N) (mem : addr -> N) : Prop :=
+Definition time_of_vTaskSwitchContext (t : trace) (gp : N) (mem : memory) : Prop :=
     (* is the scheduler suspended *)
     if (uxSchedulerSuspended gp mem) =? 0 then
         cycle_count_of_trace t = (* total number of cycles equals... *)
@@ -257,9 +273,11 @@ Definition time_of_vTaskSwitchContext (t : trace) (gp : N) (mem : addr -> N) : P
    in the proof (anything not in an invariant is forgotten after a branch).
    The properties that we state help us prove the postcondition. We must prove
    each invariant throughout the proof. *)
-Definition vTaskSwitchContext_timing_invs (_ : store) (p : addr) 
-    (base_sp gp : N) (base_mem : addr -> N) (t:trace) : option Prop :=
-match t with (Addr a, s) :: t' => match a with
+Definition vTaskSwitchContext_timing_invs (p : addr) 
+    (base_sp gp : N) (base_mem : memory) (t:trace) : option Prop :=
+match t with (Addr a, s) :: t' =>
+    let mem := s V_MEM32 in
+    match a with
     (* vApplicationStackOverflowHook *)
     (* NOTE : This function intentionally goes into an infinite loop when a
        stack overflow is detected.
@@ -268,93 +286,48 @@ match t with (Addr a, s) :: t' => match a with
     | 0x8000e804 => Some True
     (* vTaskSwitchContext *)
     | 0x80001380 => Some (
-        exists mem, s V_MEM32 = Ⓜmem /\ s R_GP = Ⓓgp /\ s R_SP = Ⓓbase_sp 
-            /\ s R_A4 = Ⓓ(uxSchedulerSuspended gp base_mem) /\
-            common_noverlaps gp base_sp mem /\
-            mem4_mem4_noverlap_stackframe gp base_sp mem /\
-            mem4_mem4_noverlap_static gp mem /\
-            ~ overlap 32
-                (gp ⊖ 920 ⊕ (31 ⊖ clz (uxTopReadyPriority gp mem) 32) * 20) 4
-                (4 + mem Ⓓ[ gp ⊖ 920 ⊕ (31 ⊖ clz (uxTopReadyPriority gp mem) 32) * 20 ] ) 4 /\
-            ~ overlap 32
-                (gp ⊖ 920 ⊕ (31 ⊖ clz (uxTopReadyPriority gp mem) 32) * 20) 4
-                (mem Ⓓ[4 + mem Ⓓ[ gp ⊖ 920 ⊕ (31 ⊖ clz (uxTopReadyPriority gp mem) 32) * 20 ]]) 4 /\
+        s R_GP = gp /\ s R_SP = base_sp 
+            /\ s R_A4 = uxSchedulerSuspended gp base_mem /\
+            memory_well_formed gp base_sp mem /\
             uxTopReadyPriority gp mem = uxTopReadyPriority gp base_mem /\
             mem Ⓓ[ 4 + mem Ⓓ[ gp ⊖ 920 + (31 ⊖ clz (uxTopReadyPriority gp mem) 32) * 20 ] ] =
             base_mem Ⓓ[ 4 + base_mem Ⓓ[ gp ⊖ 920 + (31 ⊖ clz (uxTopReadyPriority gp base_mem) 32) * 20 ] ]  /\
         cycle_count_of_trace t' = time_mem)
-    | 0x800013b4 => Some (exists mem, s V_MEM32 = Ⓜmem /\ 
-        s R_GP = Ⓓgp /\
-        common_noverlaps gp base_sp mem /\
-        mem4_mem4_noverlap_stackframe gp base_sp mem /\
-        mem4_mem4_noverlap_static gp mem /\
-        ~ overlap 32
-            (gp ⊖ 920 ⊕ (31 ⊖ clz (uxTopReadyPriority gp mem) 32) * 20) 4
-            (4 + mem Ⓓ[ gp ⊖ 920 ⊕ (31 ⊖ clz (uxTopReadyPriority gp mem) 32) * 20 ] ) 4 /\
-        ~ overlap 32
-            (gp ⊖ 920 ⊕ (31 ⊖ clz (uxTopReadyPriority gp mem) 32) * 20) 4
-            (mem Ⓓ[4 + mem Ⓓ[ gp ⊖ 920 ⊕ (31 ⊖ clz (uxTopReadyPriority gp mem) 32) * 20 ]]) 4 /\
+    | 0x800013b4 => Some (s R_GP = gp /\
+        memory_well_formed gp base_sp mem /\
         uxTopReadyPriority gp mem = uxTopReadyPriority gp base_mem /\
         mem Ⓓ[ 4 + mem Ⓓ[ gp ⊖ 920 + (31 ⊖ clz (uxTopReadyPriority gp mem) 32) * 20 ] ] =
             base_mem Ⓓ[ 4 + base_mem Ⓓ[ gp ⊖ 920 + (31 ⊖ clz (uxTopReadyPriority gp base_mem) 32) * 20 ] ]  /\
         (uxSchedulerSuspended gp base_mem =? 0) = true /\
         cycle_count_of_trace t' = 6 + 7 * time_mem + time_branch)
-    | 0x800013bc => Some (exists mem, s V_MEM32 = Ⓜmem /\ 
-        s R_GP = Ⓓgp /\
-        common_noverlaps gp base_sp mem /\
-        mem4_mem4_noverlap_stackframe gp base_sp mem /\
-        mem4_mem4_noverlap_static gp mem /\
-        ~ overlap 32
-            (gp ⊖ 920 ⊕ (31 ⊖ clz (uxTopReadyPriority gp mem) 32) * 20) 4
-            (4 + mem Ⓓ[ gp ⊖ 920 ⊕ (31 ⊖ clz (uxTopReadyPriority gp mem) 32) * 20 ] ) 4 /\
-        ~ overlap 32
-            (gp ⊖ 920 ⊕ (31 ⊖ clz (uxTopReadyPriority gp mem) 32) * 20) 4
-            (mem Ⓓ[4 + mem Ⓓ[ gp ⊖ 920 ⊕ (31 ⊖ clz (uxTopReadyPriority gp mem) 32) * 20 ]]) 4 /\
+    | 0x800013bc => Some (s R_GP = gp /\
+        memory_well_formed gp base_sp mem /\
         uxTopReadyPriority gp mem = uxTopReadyPriority gp base_mem /\
         mem Ⓓ[ 4 + mem Ⓓ[ gp ⊖ 920 + (31 ⊖ clz (uxTopReadyPriority gp mem) 32) * 20 ] ] =
             base_mem Ⓓ[ 4 + base_mem Ⓓ[ gp ⊖ 920 + (31 ⊖ clz (uxTopReadyPriority gp base_mem) 32) * 20 ] ]  /\
         (uxSchedulerSuspended gp base_mem =? 0) = true /\
         cycle_count_of_trace t' = 9 + 8 * time_mem + time_branch)
-    | 0x800013c4 => Some (exists mem, s V_MEM32 = Ⓜmem /\ 
-        s R_GP = Ⓓgp /\
-        common_noverlaps gp base_sp mem /\
-        mem4_mem4_noverlap_stackframe gp base_sp mem /\
-        mem4_mem4_noverlap_static gp mem /\
-        ~ overlap 32
-            (gp ⊖ 920 ⊕ (31 ⊖ clz (uxTopReadyPriority gp mem) 32) * 20) 4
-            (4 + mem Ⓓ[ gp ⊖ 920 ⊕ (31 ⊖ clz (uxTopReadyPriority gp mem) 32) * 20 ] ) 4 /\
-        ~ overlap 32
-            (gp ⊖ 920 ⊕ (31 ⊖ clz (uxTopReadyPriority gp mem) 32) * 20) 4
-            (mem Ⓓ[4 + mem Ⓓ[ gp ⊖ 920 ⊕ (31 ⊖ clz (uxTopReadyPriority gp mem) 32) * 20 ]]) 4 /\
+    | 0x800013c4 => Some (s R_GP = gp /\
+        memory_well_formed gp base_sp mem /\
         uxTopReadyPriority gp mem = uxTopReadyPriority gp base_mem /\
         mem Ⓓ[ 4 + mem Ⓓ[ gp ⊖ 920 + (31 ⊖ clz (uxTopReadyPriority gp mem) 32) * 20 ] ] =
             base_mem Ⓓ[ 4 + base_mem Ⓓ[ gp ⊖ 920 + (31 ⊖ clz (uxTopReadyPriority gp base_mem) 32) * 20 ] ]  /\
         (uxSchedulerSuspended gp base_mem =? 0) = true /\
         cycle_count_of_trace t' = 12 + 9 * time_mem + time_branch
     )
-    | 0x800013cc => Some (exists mem, s V_MEM32 = Ⓜmem /\ 
-        s R_GP = Ⓓgp /\
-        common_noverlaps gp base_sp mem /\
-        mem4_mem4_noverlap_stackframe gp base_sp mem /\
-        mem4_mem4_noverlap_static gp mem /\
-        ~ overlap 32
-            (gp ⊖ 920 ⊕ (31 ⊖ clz (uxTopReadyPriority gp mem) 32) * 20) 4
-            (4 + mem Ⓓ[ gp ⊖ 920 ⊕ (31 ⊖ clz (uxTopReadyPriority gp mem) 32) * 20 ] ) 4 /\
-        ~ overlap 32
-            (gp ⊖ 920 ⊕ (31 ⊖ clz (uxTopReadyPriority gp mem) 32) * 20) 4
-            (mem Ⓓ[4 + mem Ⓓ[ gp ⊖ 920 ⊕ (31 ⊖ clz (uxTopReadyPriority gp mem) 32) * 20 ]]) 4 /\
+    | 0x800013cc => Some (s R_GP = gp /\
+        memory_well_formed gp base_sp mem /\
         uxTopReadyPriority gp mem = uxTopReadyPriority gp base_mem /\
         mem Ⓓ[ 4 + mem Ⓓ[ gp ⊖ 920 + (31 ⊖ clz (uxTopReadyPriority gp mem) 32) * 20 ] ] =
             base_mem Ⓓ[ 4 + base_mem Ⓓ[ gp ⊖ 920 + (31 ⊖ clz (uxTopReadyPriority gp base_mem) 32) * 20 ] ]  /\
         (uxSchedulerSuspended gp base_mem =? 0) = true /\
         cycle_count_of_trace t' = 15 + 10 * time_mem + time_branch
     )
-    | 0x80001418 => Some (exists mem, s V_MEM32 = Ⓜmem /\ 
-        s R_GP = Ⓓgp /\
-        s R_A1 = Ⓓ(mem Ⓓ[4 + (gp ⊖ 924) ⊕ ((31 ⊖ (clz (uxTopReadyPriority gp mem) 32)) * 20)]) /\
-        s R_A2 = Ⓓ(addr_pxReadyTasksLists gp ⊕ ((31 ⊖ (clz (uxTopReadyPriority gp mem) 32)) * 20)) /\
-        s R_A5 = Ⓓ((gp ⊖ 916) ⊕ (31 ⊖ clz (uxTopReadyPriority gp mem) 32) * 20) /\
-        common_noverlaps gp base_sp mem /\
+    | 0x80001418 => Some (s R_GP = gp /\
+        s R_A1 = mem Ⓓ[4 + (gp ⊖ 924) ⊕ ((31 ⊖ (clz (uxTopReadyPriority gp mem) 32)) * 20)] /\
+        s R_A2 = addr_pxReadyTasksLists gp ⊕ ((31 ⊖ (clz (uxTopReadyPriority gp mem) 32)) * 20) /\
+        s R_A5 = (gp ⊖ 916) ⊕ (31 ⊖ clz (uxTopReadyPriority gp mem) 32) * 20 /\
+        memory_well_formed gp base_sp mem /\
         uxTopReadyPriority gp mem = uxTopReadyPriority gp base_mem /\
         mem Ⓓ[ gp ⊖ 920 + (31 ⊖ clz (uxTopReadyPriority gp mem) 32) * 20 ] =
             base_mem Ⓓ[ 4 + base_mem Ⓓ[ gp ⊖ 920 + (31 ⊖ clz (uxTopReadyPriority gp base_mem) 32) * 20 ] ]  /\
@@ -411,6 +384,9 @@ Ltac find_rewrites :=
         rewrite H
     end).
 
+(* Override some function call behavior - TODO : fix *)
+Ltac generalize_trace ::= idtac.
+
 (* We use simpl in a few convenient places: make sure it doesn't go haywire *)
 Arguments N.add _ _ : simpl nomatch.
 Arguments N.mul _ _ : simpl nomatch.
@@ -422,79 +398,72 @@ Theorem vTaskSwitchContext_timing:
   forall s p t s' x' gp sp mem
          (ENTRY: startof t (x',s') = (Addr start_vTaskSwitchContext,s))
          (MDL: models rvtypctx s)
-         (GP : s R_GP = Ⓓgp)
-         (SP : s R_SP = Ⓓsp)
-         (MEM : s V_MEM32 = Ⓜmem)
-         (NOVERLAPS : common_noverlaps gp sp mem)
-         (MEM4_NOVERLAPS : 
-            mem4_mem4_noverlap_stackframe gp sp mem /\
-            mem4_mem4_noverlap_static gp mem /\
-            ~ overlap 32
-                (gp ⊖ 920 ⊕ (31 ⊖ clz (uxTopReadyPriority gp mem) 32) * 20) 4
-                (4 + mem Ⓓ[ gp ⊖ 920 ⊕ (31 ⊖ clz (uxTopReadyPriority gp mem) 32) * 20 ] ) 4 /\
-            ~ overlap 32
-                (gp ⊖ 920 ⊕ (31 ⊖ clz (uxTopReadyPriority gp mem) 32) * 20) 4
-                (mem Ⓓ[4 + mem Ⓓ[ gp ⊖ 920 ⊕ (31 ⊖ clz (uxTopReadyPriority gp mem) 32) * 20 ]]) 4)
-         ,
+         (GP : s R_GP = gp)
+         (SP : s R_SP = sp)
+         (MEM : s V_MEM32 = mem)
+         (NOVERLAPS : memory_well_formed gp sp mem),
   satisfies_all 
     lifted_vTaskSwitchContext                                 (* Provide lifted code *)
-    (vTaskSwitchContext_timing_invs s p sp gp mem)            (* Provide invariant set *)
+    (vTaskSwitchContext_timing_invs p sp gp mem)            (* Provide invariant set *)
     vTaskSwitchContext_exit                                   (* Provide exit point *)
   ((x',s')::t).
 Proof using.
     (* Set up our proof environment *)
     intros.
     apply prove_invs.
-    Local Ltac step := time rv_step.
+    Local Ltac step := time r5_step.
 
     Local Ltac unfold_vTaskSwitchContext :=
         unfold uxSchedulerSuspended, __global_size,
         vTaskSwitchContext_stack_frame_size, uxSchedulerSuspended,
-        gp_sp_noverlap, smem_well_formed, pxCurrentTCB_noverlap_static,
-        pxCurrentTCB_noverlap_stackframe, pxCurrentTCB_noverlap_clz_static,
-        clz_noverlap_smem, mem_pxCurrentTCB_noverlap_stackframe,
-        mem_pxCurrentTCB_noverlap_static, offset_mem_pxCurrentTCB_noverlap_clz,
-        mem4_mem4_noverlap_static, mem4_mem4_noverlap_stackframe,
-        clz_noverlap_sframe, mem4_pxCurrentTCB_noverlap_stackframe,
-        mem4_pxCurrentTCB_noverlap_static, pxCurrentTCB, uxTopReadyPriority,
+        pxCurrentTCB, uxTopReadyPriority,
         addr_pxReadyTasksLists in *.
     Local Ltac noverlap_prepare gp sp := 
         _noverlap_prepare unfold_vTaskSwitchContext gp sp.
-    Local Ltac destruct_noverlaps :=
+    Local Ltac unfold_mem_wf :=
         match goal with
-        | [H: common_noverlaps _ _ _ |- _] =>
-            destruct H as [GP_SP_FAR [SMEM_WELL_FORMED [PCT_NOL_STATIC 
-            [PCT_NOL_SFRAME [PCT_NOL_CLZ [CLZ_NOL_STATIC 
-            [MEM_PCT_NOL_SFRAME [MEM_PCT_NOL_STATIC [OFF_MEM_PCT_NOL_CLZ
-            [CLZ_NOL_SFRAME [MEM4_PCT_NOL_SFRAME MEM4_PCT_NOL_STATIC]]]]]]]]]]]
-        end. 
-    destruct_noverlaps.
+        | [H: memory_well_formed _ _ _ |- _] =>
+            unfold memory_well_formed in H;
+            destruct H as [SMEM_WF NOVERLAPS]
+        end.
+    unfold_mem_wf.
 
     (* Base case *)
-    simpl. rewrite ENTRY. step.
-    destruct MEM4_NOVERLAPS, H0, H1. unfold uxSchedulerSuspended, msub.
-    handle_ex; now psimpl.
+    simpl. rewrite ENTRY. step. now repeat split.
 
     (* Inductive step setup *)
     intros.
     eapply startof_prefix in ENTRY; try eassumption.
     eapply preservation_exec_prog in MDL; 
         try eassumption; [idtac|apply lift_riscv_welltyped].
-    clear - ENTRY PRE MDL. rename t1 into t. rename s1 into s'. 
+    clear - PRE MDL. rename t1 into t. rename s1 into s.
     rename mem into base_mem.
 
     (* Meat of proof starts here *)
     destruct_inv 32 PRE.
 
     (* 0x800015e4 *)
-    destruct PRE as (mem & MEM & GP & SP & A4 & NOVERLAPS & MEM4_MEM4_NOL_SFRAME
-        & MEM4_MEM4_NOL_STATIC & MEM4_920 & MEM4_MEM4_920 & PreservesPriority
-        & Preserves920 & Cycles). destruct_noverlaps.
+    destruct PRE as (GP & SP & A4 & MWF & PreservesPriority & Preserves920).
+    unfold_mem_wf.
     repeat step. handle_ex.
-        1-10: noverlap_prepare gp sp; memsolve mem gp sp.
-        1-5: noverlap_prepare gp sp; memsolve mem gp sp;
+    {
+        unfold smem_well_formed. intros.
+        unfold non_overlapping_smem_layout, uxTopReadyPriority in H0, H1.
+        rewrite getmem_noverlap in H0, H1.
+        rewrite getmem_noverlap in H0, H1.
+        rewrite getmem_noverlap in H0, H1.
+        simpl in H0, H1.
+
+        destruct H0. inversion H0; subst x xw.
+            destruct H1. inversion H1; subst y yw. contradiction.
+            destruct H1. inversion H1; subst y yw.
+            - apply SMEM_WF. psimpl.
+        admit.
+    }
+
+        par: try solve [noverlap_prepare gp sp; memsolve mem gp sp;
             try now eapply MEM4_PCT_NOL_STATIC;
-            eauto using noverlap_symmetry.
+            eauto using noverlap_symmetry].
         {
             noverlap_prepare gp sp.
             repeat rewrite <- getmem_mod_l with (a := _ + _).
